\documentclass[fleqn]{article}
\usepackage{amsmath}


\title{Double Ring Ising model}
\author{Shane Harding}

\date{\today}


\begin{document}
\maketitle

Define the 4 possible spins as $s_i$ where

\[ s_i \in \left\{ \left( \begin{array}{c} +1 \\ +1 \end{array} \right),
\left( \begin{array}{c} +1 \\ -1 \end{array} \right),
\left( \begin{array}{c} -1 \\ +1 \end{array} \right),
\left( \begin{array}{c} -1 \\ -1 \end{array} \right) \right\} \]

The Hamiltonian is given by:

\[ H = -J \sum_{\langle i, j \rangle} s_i \cdot s_j \]

we set $J=1$ for simplicity and take the dot product of the two spin vectors. The partition function, $Z$, is given by the trace of the matrix $P$ which has entries $e^{H(s_i, s_j)}$ for all possible combinations of $s_i, s_j$.

\begin{align}
P &=& \left( \begin{array}{cccc} e^{-2 \beta} & e^0 & e^0 & e^{2 \beta} \\
e^0 & e^{-2 \beta} & e^{2 \beta} & e^0 \\
e^0 & e^{2 \beta} & e^{-2 \beta} & e^0 \\
e^{2 \beta} & e^0 & e^0 & e^{-2 \beta} \end{array} \right) \\
%%%
&=& \left( \begin{array}{cccc} e^{-2 \beta} & 1 & 1 & e^{2 \beta} \\
1 & e^{-2 \beta} & e^{2 \beta} & 1 \\
1 & e^{2 \beta} & e^{-2 \beta} & 1 \\
e^{2 \beta} & 1 & 1 & e^{-2 \beta} \end{array} \right) \\
\end{align}

Now find the eigenvalues.. $det(P-\lambda I)$.

\begin{eqnarray}
\left| \begin{array}{cccc} e^{-2 \beta} - \lambda & 1 & 1 & e^{2 \beta} \\
1 & e^{-2 \beta} - \lambda & e^{2 \beta} & 1 \\
1 & e^{2 \beta} & e^{-2 \beta} - \lambda & 1 \\
e^{2 \beta} & 1 & 1 & e^{-2 \beta} - \lambda \end{array} \right| \\
\end{eqnarray}

\begin{eqnarray}
= (e^{-2 \beta} - \lambda) \left| \begin{array}{ccc} e^{-2 \beta} - \lambda & e^{2 \beta} & 1  \\
e^{2 \beta} & e^{-2 \beta} - \lambda & 1 \\
1 & 1 & e^{-2 \beta} - \lambda  \end{array} \right| 
%%
- \left| \begin{array}{ccc} 1 & e^{2 \beta} & 1 \\
1 & e^{-2 \beta} - \lambda & 1 \\
e^{2 \beta} & 1 & e^{-2 \beta} - \lambda  \end{array} \right| \\
%%
+ \left| \begin{array}{ccc} 1 & e^{-2 \beta} - \lambda & 1 \\
1 & e^{2 \beta} & 1 \\
e^{2 \beta} & 1 & e^{-2 \beta} - \lambda  \end{array} \right| 
%%
-e^{2 \beta} \left| \begin{array}{ccc} 1 & e^{-2 \beta} - \lambda & e^{2 \beta} \\
1 & e^{2 \beta} & e^{-2 \beta} - \lambda \\
e^{2 \beta} & 1 & 1  \end{array} \right| \\
%%%%%%%%%%
= (e^{-2 \beta} - \lambda) \left[ (e^{-2 \beta} - \lambda) \left( (e^{-2 \beta} - \lambda)^2 - 1 \right) - e^{2 \beta} \left( e^{2 \beta} (e^{-2 \beta} - \lambda) - 1 \right) + (e^{2 \beta} - (e^{-2 \beta} - \lambda) ) \right] \\
%%
- \left[ \left( (e^{-2 \beta} - \lambda)^2 -1 \right) - \left( e^{2 \beta} (e^{-2 \beta} - \lambda) - 1 \right) + e^{2 \beta} \left( e^{2 \beta} - (e^{-2 \beta} - \lambda) \right) \right] \\
%%
 + \left[ e^{2 \beta} \left( (e^{-2 \beta} - \lambda) - 1 \right) - \left( (e^{-2 \beta} - \lambda)^2 -1 \right) + e^{2 \beta} \left( (e^{-2 \beta} - \lambda) - e^{2 \beta} \right) \right] \\
%%
- e^{2 \beta} \left[ \left( e^{2 \beta} - (e^{-2 \beta} - \lambda) \right) - \left( (e^{-2 \beta} - \lambda) - e^{2 \beta} \right) + e^{2 \beta} \left( (e^{-2 \beta} - \lambda)^2 - e^{4 \beta} \right) \right] \\
%%%%%%%%%
= (e^{-2 \beta} - \lambda) \left[ (e^{-2 \beta} - \lambda)^3 - (e^{-2 \beta} - \lambda) - e^{4 \beta} (e^{-2 \beta} - \lambda) + e^{2 \beta} + e^{2 \beta} - (e^{-2 \beta} - \lambda) \right] \\
%%
- \left[ (e^{-2 \beta} - \lambda) -1 -e^{2 \beta} (e^{-2 \beta} - \lambda) +1 - e^{2 \beta} (e^{-2 \beta} - \lambda) + e^{4 \beta} \right] \\
%%
+ \left[ e^{2 \beta} (e^{-2 \beta} - \lambda) - e^{2 \beta} - (e^{-2 \beta} - \lambda)^2 + 1 + e^{2 \beta} (e^{-2 \beta} - \lambda) - e^{4 \beta} \right] \\
%%
- e^{2 \beta} \left[ e^{2 \beta} - (e^{-2 \beta} - \lambda) - (e^{-2 \beta} - \lambda) + e^{2 \beta} + e^{2 \beta} (e^{-2 \beta} - \lambda) - e^{6 \beta} \right] \\
%%%%%%%%
= (e^{-2 \beta} - \lambda)^4 - 2 (e^{-2 \beta} - \lambda)^2 - e^{4 \beta}(e^{-2 \beta} - \lambda)^2 + 2 e^{2 \beta} (e^{-2 \beta} - \lambda) - (e^{-2 \beta} - \lambda)^2 \\
 + 2 e^{2 \beta} (e^{-2 \beta} - \lambda) - e^{4 \beta} + 2 e^{2 \beta} (e^{-2 \beta} - \lambda) - (e^{-2 \beta} - \lambda)^2 \\
-e^{2 \beta} +1 -2 e^{4 \beta} - e^{4 \beta} + 2 e^{2 \beta} (e^{-2 \beta} - \lambda) - e^{4 \beta} (e^{-2 \beta} - \lambda)^2 + e^{8 \beta}
\end{eqnarray}





\end{document}
